[minor] RefinementQAC compiles again.
Changed the notion of initial data for the concrete machine. It now
includes the whole concrete memory. This requires us to place some
additional hypothesis when matching initial data, but it doesn't seem
too bad.

pico-ifc-coq/dyn_allocation/RefinementQAC.v
@@ -1200,19 +1200,25 @@ Proof.
       eapply kernel_run_success_fail_contra; eauto.
 Qed.
 
+Definition ac_match_initial_stack_data stkdata1 stkdata2 mem :=
+  Forall2 (fun a1 a2 => pcatom_labToZ a1 a2 mem) stkdata1 stkdata2.
+
 Inductive ac_match_initial_data :
   abstract_init_data T ->
   init_data (concrete_machine cblock faultHandler) -> Prop :=
-| ac_mid : forall d1 p1 b1,
+| ac_mid : forall prog mem stkdata1 stkdata2 def1 def2
+                  (UP2DATE : cache_up2date mem)
+                  (DATA : ac_match_initial_stack_data stkdata1 stkdata2 mem)
+                  (DEF : labToZ def1 def2 mem),
              ac_match_initial_data
-               (p1, d1, b1)
-               (p1, map pcatom_labToZ d1, labToZ b1).
+               (prog, stkdata1, def1)
+               (prog, mem, stkdata2, def2).
 
 (* Maybe move this later *)
 Definition emptyinj : meminj := fun _ => None.
 Hint Unfold emptyinj.
 
-Lemma emptyinj_meminj : Meminj (Mem.empty _ _) (initial_memory cblock) emptyinj.
+Lemma emptyinj_meminj : forall mem, Meminj (Mem.empty _ _) mem emptyinj.
 Proof.
   unfold emptyinj.
   constructor; simpl; congruence.
@@ -1225,26 +1231,18 @@ Proof.
 Qed.
 Hint Resolve emptyinj_userinj.
 
-Lemma match_init_stacks: forall d1,
- match_stacks emptyinj
-              (map (fun a : PcAtom T => let (i,l) := a in AData (Vint i,l)) d1)
-              (map (fun a : PcAtom Z => let (i,l) := a in CData (Vint i,l)) (map pcatom_labToZ d1)).
+Lemma match_init_stacks:
+  forall stkdata1 stkdata2 mem
+         (STKDATA : ac_match_initial_stack_data stkdata1 stkdata2 mem),
+    match_stacks emptyinj
+                 (map (fun a : PcAtom T => let (i,l) := a in AData (Vint i,l)) stkdata1)
+                 (map (fun a : PcAtom Z => let (i,l) := a in CData (Vint i,l)) stkdata2) mem.
 Proof.
-  induction d1 as [|[xv xl] d1 IH]; intros;
-  repeat (simpl; constructor; auto).
+  induction 1 as [|[xv1 xl1] [xv2 xl2] sd1 sd2 [H1 H2]];
+  intros;
+  repeat (simpl in *; subst; constructor; auto).
 Qed.
 Hint Resolve match_init_stacks.
-
-Lemma initial_memory_up2date :
-  cache_up2date (initial_memory cblock).
-Proof.
-  econstructor; eauto using Mem.get_init_eq.
-  intros opcode vls pcl contra.
-  inv contra.
-  inv OP.
-  inv H.
-Qed.
-Hint Resolve initial_memory_up2date.
 
 Lemma ac_match_initial_data_match_initial_states :
   forall ai ci,
@@ -1358,10 +1356,6 @@ Proof.
     inv H.
   - exploit cache_hit_simulation; eauto.
     intros [e1 [s1' [STEP [ME MS]]]].
-    unfold match_events in *. subst.
-    (*assert (exists t', t = filter (@is_event _) t') by
-        (destruct (concretize_event e1); eauto using filter_cons_inv).*)
-    (*inv H2.*)
     exploit IHEXEC; eauto.
     intros [t1 [? [? ?]]].
     exists (op_cons e1 t1). eexists.
